src/translate.ml
@@ -2,7 +2,7 @@ open Fsm
 
 let to_fsm (lts : Lts.lts) : fsm =
   match lts with
-  | { init = _init; transitions; is_complete } ->
+  | { init = _init; transitions; info } ->
     let init : state =
       Create.state
         (Of
@@ -13,12 +13,7 @@ let to_fsm (lts : Lts.lts) : fsm =
     in
     let states : States.t = States.singleton init in
     let fsm : fsm =
-      Create.fsm
-        ~is_complete
-        (Some init)
-        (Create.alphabet ())
-        states
-        (Edges.create 0)
+      Create.fsm ~info (Some init) (Create.alphabet ()) states (Edges.create 0)
     in
     Lts.Transitions.fold
       (fun (t : Lts.transition) (acc : fsm) ->
